proofs/fstar/extraction/Libcrux.Kem.Kyber.Hash_functions.fsti
@@ -18,6 +18,9 @@ type t_XofState =
 val v_XOF_absorb (v_K: usize) (input: t_Array (t_Array u8 (sz 34)) v_K)
     : Prims.Pure t_XofState Prims.l_True (fun _ -> Prims.l_True)
 
+val v_XOF_free (v_K: usize) (xof_state: t_XofState)
+    : Prims.Pure Prims.unit Prims.l_True (fun _ -> Prims.l_True)
+
 val v_XOF_squeeze_block (v_K: usize) (xof_state: t_XofState)
     : Prims.Pure (t_Array (t_Array u8 (sz 168)) v_K & t_XofState)
       Prims.l_True
